questions.py

TPTPAxioms/Test.hs
@@ -1,0 +1,18 @@
+import Data.TPTP
+import Data.TPTP.Parse.Text
+import Data.TPTP.Pretty
+import Data.Text
+
+test :: Text
+test =
+    pack
+        "cnf(member_of_union_is_member_of_one_set,axiom,\
+        \( ~ union(Set1,Set2,Union)\
+        \| ~ member(Element,Union)\
+        \| member(Element,Set1)\
+        \| member(Element,Set2) ) )."
+
+out :: TPTP
+out = case parseTPTPOnly test of
+    Left _ -> error "oops"
+    Right out -> out
