test.v
@@ -1,14 +1,271 @@
-Require Import Lia.
-Require Extraction.
+Require Import Coq.Bool.Bool.
+Require Import Coq.Init.Nat.
+Require Import Coq.Logic.FunctionalExtensionality.
 
-Lemma basic_arith : forall x y z,
-    x * (y + z) = (x * y) + (x * z).
-Proof. lia. Qed.
-Print basic_arith.
+Definition set {A : Set} := (A -> bool).
 
-Lemma simpler_arith : forall x y,
-    x + y = y + x.
-Proof. lia. Qed.
-Print simpler_arith.
+Definition setA (x : nat) :=
+  match x with
+    | 0 | 1 | 2 => true
+    | _ => false
+  end.
 
-Extraction simpler_arith.
+Definition setB (x : nat) :=
+  match x with
+    | 3 | 4 | 5 => true
+    | _ => false
+  end.
+
+Definition union {A : Set} (set1 set2 : @set A) : @set A :=
+  fun x => orb (set1 x) (set2 x).
+
+Compute ((union setA setB) 4).
+
+Definition subset {A} (set1 set2 : @set A) : Prop :=
+  forall x, set1 x = true -> set2 x = true.
+
+Theorem proof1 {A} :
+  forall x y : @set A, subset x y -> forall z, subset (union x z) (union y z).
+Proof.
+  unfold subset. unfold union. intros. apply orb_true_iff. apply orb_prop in H0. destruct H0; auto.
+Qed.
+
+Theorem proof2 {A} :
+  forall a b c : @set A, union (union a b) c = union a (union b c).
+Proof.
+  intros. unfold union. apply functional_extensionality. intros.
+  destruct (a x); auto.
+Qed.
+
+Theorem proof3 {A} :
+  forall (a b : @set A) x, a x = false /\ (union a b) x = true -> b x = true.
+Proof.
+  intros a b x [nAx ABx]. unfold union in ABx. rewrite nAx in ABx. auto.
+Qed.
+
+Theorem subset_trans {A} :
+  forall (a b c : @set A), subset a b /\ subset b c -> subset a c.
+Proof.
+  unfold subset. intros a b c [Hab Hbc] x Ha.
+  auto.
+  (* apply Hab in Ha. apply Hbc in Ha. apply Ha. *)
+Qed.
+
+Theorem subset_trans3 {A} :
+  forall (a b c d : @set A), subset a b ->
+                        subset b c ->
+                        subset c d ->
+                        subset a d.
+Proof.
+  intros. eapply subset_trans. split.
+  - apply H.
+  - eapply subset_trans. split; eauto.
+Qed.
+
+Theorem trans_app {A} :
+  forall (a b c x : @set A), subset a b ->
+                        subset b c ->
+                        subset (union a x) (union c x).
+Proof.
+  intros. assert (subset a c). { eapply subset_trans. split; eassumption. }
+  apply proof1. assumption.
+Restart.
+  intros. assert (subset (union a x) (union b x)). { apply proof1. assumption. }
+          assert (subset (union b x) (union c x)). { apply proof1. assumption. }
+  eapply subset_trans. split; eassumption.
+Qed.
+
+Structure group :=
+  {
+    G :> Set;
+
+    id : G;
+    op : G -> G -> G;
+    inv : G -> G;
+
+    op_assoc : forall (x y z : G), op x (op y z) = op (op x y) z;
+    op_inv_l : forall (x : G), id = op (inv x) x;
+    op_inv_r : forall (x : G), id = op x (inv x);
+    op_id_l : forall (x : G), x = op id x;
+    op_id_r : forall (x : G), x = op x id;
+  }.
+
+Arguments id {g}.
+Arguments op {g} _ _.
+Arguments inv {g} _.
+
+Hint Resolve op_assoc : groups.
+Hint Resolve op_inv_l : groups.
+Hint Resolve op_inv_r : groups.
+Hint Resolve op_id_l : groups.
+Hint Resolve op_id_r : groups.
+
+Fixpoint exp (G : group) (x : G) (n : nat) : G :=
+  match n with
+    | O => id
+    | S n' => op x (exp G x n')
+  end.
+Arguments exp {G} _ _.
+
+Notation "x <.> y" := (op x y) (at level 50, left associativity).
+Notation "x ** n" := (exp x n) (at level 50, left associativity).
+
+Lemma right_mul :
+  forall (G : group) (x y z : G),
+    x = y ->
+    x <.> z = y <.> z.
+Proof. intros. auto. rewrite H. reflexivity. Qed.
+
+Lemma left_mul :
+  forall (G : group) (x y z : G),
+    x = y ->
+    z <.> x = z <.> y.
+Proof. intros. rewrite H. reflexivity. Qed.
+
+Lemma right_mul' :
+  forall (G : group) (x y z : G),
+    x <.> z = y <.> z ->
+    x = y.
+Proof.
+  intros.
+  apply right_mul with (z := inv z) in H.
+  repeat rewrite <- op_assoc in H.
+  repeat rewrite <- op_inv_r in H.
+  repeat rewrite <- op_id_r in H.
+  apply H.
+Qed.
+
+Lemma left_mul' :
+  forall (G : group) (x y z : G),
+    z <.> x = z <.> y ->
+    x = y.
+Proof.
+  intros. apply left_mul with (z := inv z) in H.
+  repeat rewrite op_assoc in H.
+  repeat rewrite <- op_inv_l in H.
+  repeat rewrite <- op_id_l in H.
+  apply H.
+Qed.
+
+Lemma ab_inv :
+  forall (G : group) (a b : G), inv (a <.> b) = (inv b) <.> (inv a).
+Proof.
+  intros. apply right_mul' with (z := a).
+  rewrite <- op_assoc. rewrite <- op_inv_l. rewrite <- op_id_r.
+  apply right_mul' with (z := b). rewrite <- op_inv_l.
+  rewrite <- op_assoc. rewrite <- op_inv_l. reflexivity.
+Qed.
+
+Lemma mul_exp_eq_add :
+  forall (G : group) (x : G) (n m : nat),
+    x ** (n + m) = (x ** n) <.> (x ** m).
+Proof with auto with groups.
+  intros. induction n.
+  - simpl...
+  - simpl. rewrite IHn...
+Qed.
+
+Lemma add_comm : forall a b, a + b = b + a.
+Proof. intros. induction a.
+       - trivial.
+       - simpl. rewrite IHa. rewrite plus_n_Sm. reflexivity.
+Qed.
+
+Lemma exp_commute :
+  forall (G : group) (x : G) (n m : nat),
+    (x ** n) <.> (x ** m) = (x ** m) <.> (x ** n).
+Proof.
+  intros. rewrite <- mul_exp_eq_add.
+  rewrite add_comm.
+  rewrite mul_exp_eq_add. reflexivity.
+Qed.
+
+Lemma stack_exp_eq_mul :
+  forall (G : group) (x : G) (n m : nat),
+    (x ** n) ** m = x ** (n * m).
+Proof.
+  intros. induction m.
+  - simpl. induction n.
+    + simpl. reflexivity.
+    + simpl. assumption.
+  - simpl. rewrite IHm.
+    rewrite <- mult_n_Sm. rewrite mul_exp_eq_add.
+    rewrite exp_commute. reflexivity.
+Qed.
+
+Lemma id_exp_eq_id : forall (G : group) (n : nat), @id G ** n = id.
+Proof.
+  induction n.
+  - trivial.
+  - simpl. rewrite IHn. auto with groups.
+Qed.
+
+Lemma ord2_impl_inv :
+  forall (G : group) (x : G), x <.> x = id ->
+                         x = inv x.
+Proof.
+  intros. apply left_mul' with (z := x). rewrite <- op_inv_r.
+  apply H.
+Qed.
+
+Lemma ord2_impl_abel :
+  forall (G : group), (forall x : G, x <.> x = id) ->
+                 (forall x y : G, x <.> y = y <.> x).
+Proof.
+  intros. set (Hactive := H).
+  specialize Hactive with (x <.> y).
+  apply ord2_impl_inv in Hactive.
+  rewrite ab_inv in Hactive.
+  set (Hx := H). specialize Hx with x. specialize H with y.
+  apply ord2_impl_inv in H. apply ord2_impl_inv in Hx.
+  rewrite <- H in Hactive. rewrite <- Hx in Hactive. apply Hactive.
+  Show Proof.
+Qed.
+(* Restart. *)
+(*   intros. specialize H with (x <.> y). move/ord2_impl_inv in H. *)
+(*   intros. rewrite <- H with (x := x <.> y). (* TODO: learn ssreflect *) *)
+
+Definition has_order (G : group) (x : G) (n : nat) : Prop :=
+  x ** n = id /\ ~(exists m, 0 < m < n /\ x ** m = id).
+Arguments has_order {G} _ _.
+
+Lemma div : forall m n,
+    m >= n ->
+    (* m = n * (m / n) + (m mod n). *)
+    (exists k r, m = n * k + r /\ 1 <= k /\ 0 <= r < n).
+Proof.
+Admitted.
+
+Lemma m_l_n_gt : forall n m, ~(m < n) -> m >= n.
+Admitted.
+
+Lemma fin_ord_div : forall (G : group) (x : G) (n m : nat),
+    m > 0 ->
+    has_order x n -> x ** m = id -> (exists a, m = mul n a).
+Proof.
+  unfold has_order. intros G x n m Hmp [Hn Hnmin] Hm.
+  assert (~(m < n)). {
+    unfold not. intros. apply Hnmin. exists m. auto.
+  }
+  assert (m >= n). {
+    apply m_l_n_gt. assumption.
+  }
+  apply div in H0. destruct H0 as [k [r [H0 [Hk Hr]]]]. rewrite H0 in Hm.
+  rewrite mul_exp_eq_add in Hm. rewrite <- stack_exp_eq_mul in Hm.
+  rewrite Hn in Hm. rewrite id_exp_eq_id in Hm.
+  rewrite <- op_id_l in Hm.
+  assert (~(r > 0)). {
+    unfold not. intros. apply Hnmin. exists r. split.
+    - split.
+      + auto.
+      + destruct Hr. assumption.
+    - assumption.
+  }
+  assert (r = 0). {
+    induction r.
+    - reflexivity.
+    - exfalso. apply H1. unfold gt. unfold lt. apply le_n_S. apply le_0_n.
+  }
+  rewrite H2 in H0. rewrite <- plus_n_O in H0. exists k. assumption.
+  Show Proof.
+Qed.
